<?xml version="1.0" encoding="utf-8"?>
<rdf:RDF
  xmlns:owl="http://www.w3.org/2002/07/owl#"
  xmlns:dc="http://purl.org/dc/elements/1.1/"
  xmlns:rdfs="http://www.w3.org/2000/01/rdf-schema#"
  xmlns:rdf="http://www.w3.org/1999/02/22-rdf-syntax-ns#"
>
  <owl:AnnotationProperty rdf:about="https://bamresearch.github.io/bam-masterdata/dataType">
    <rdfs:label xml:lang="en">bam:dataType</rdfs:label>
    <rdfs:comment xml:lang="en">Represents the data type of a property as defined in the openBIS platform.
        This annotation is used to ensure alignment with the native data types in openBIS,
        facilitating seamless integration and data exchange.

        The allowed values for this annotation correspond directly to the openBIS type system,
        including BOOLEAN, CONTROLLEDVOCABULARY, DATE, HYPERLINK, INTEGER, MULTILINE_VARCHAR, OBJECT,
        REAL, TIMESTAMP, VARCHAR, and XML.

        While `bam:dataType` is primarily intended for internal usage with openBIS, mappings to
        standard vocabularies such as `xsd` (e.g., `xsd:boolean`, `xsd:string`) are possible to use and documented to
        enhance external interoperability. The full mapping is:
        - BOOLEAN: xsd:boolean
        - CONTROLLEDVOCABULARY: xsd:string
        - DATE: xsd:date
        - HYPERLINK: xsd:anyURI
        - INTEGER: xsd:integer
        - MULTILINE_VARCHAR: xsd:string
        - OBJECT: bam:ObjectType
        - REAL: xsd:decimal
        - TIMESTAMP: xsd:dateTime
        - VARCHAR: xsd:string
        - XML: xsd:string</rdfs:comment>
  </owl:AnnotationProperty>
  <owl:ObjectProperty rdf:about="https://bamresearch.github.io/bam-masterdata/referenceTo">
    <rdfs:domain>
      <owl:Thing rdf:about="https://bamresearch.github.io/bam-masterdata/PropertyType">
        <rdfs:label xml:lang="en">PropertyType</rdfs:label>
        <rdfs:comment xml:lang="en">A conceptual placeholder used to define and organize properties as first-class entities.
        PropertyType is used to place properties and define their metadata, separating properties from the
        entities they describe.

        In integration scenarios:
        - PropertyType can align with `BFO:Quality` for inherent attributes.
        - PropertyType can represent `BFO:Role` if properties serve functional purposes.
        - PropertyType can be treated as a `prov:Entity` when properties participate in provenance relationships.</rdfs:comment>
      </owl:Thing>
    </rdfs:domain>
    <rdfs:label xml:lang="en">referenceTo</rdfs:label>
    <rdfs:comment xml:lang="en">The property is referencing an object existing in openBIS.</rdfs:comment>
  </owl:ObjectProperty>
  <owl:AnnotationProperty rdf:about="https://bamresearch.github.io/bam-masterdata/propertyLabel">
    <rdfs:label xml:lang="en">bam:propertyLabel</rdfs:label>
    <rdfs:comment xml:lang="en">A UI-specific annotation used in openBIS to provide an alternative label for a property
        displayed in the frontend. Not intended for semantic reasoning or interoperability beyond openBIS.</rdfs:comment>
  </owl:AnnotationProperty>
  <owl:Thing rdf:about="https://bamresearch.github.io/bam-masterdata/CollectionType">
    <rdfs:label xml:lang="en">CollectionType</rdfs:label>
  </owl:Thing>
  <owl:Thing rdf:about="https://bamresearch.github.io/bam-masterdata/ExampleObjectType">
    <rdfs:subClassOf>
      <owl:Thing rdf:about="https://bamresearch.github.io/bam-masterdata/ObjectType">
        <rdfs:label xml:lang="en">ObjectType</rdfs:label>
      </owl:Thing>
    </rdfs:subClassOf>
    <rdfs:subClassOf>
      <owl:Restriction rdf:nodeID="Nccb85c1b27a34863b30a5af64c2df77e">
        <owl:onProperty rdf:resource="https://bamresearch.github.io/bam-masterdata/hasMandatoryProperty"/>
        <owl:someValuesFrom rdf:resource="https://bamresearch.github.io/bam-masterdata/Name"/>
      </owl:Restriction>
    </rdfs:subClassOf>
    <rdfs:subClassOf>
      <owl:Restriction rdf:nodeID="N9a5975fcd1234108a5cf1df671c46e5d">
        <owl:onProperty rdf:resource="https://bamresearch.github.io/bam-masterdata/hasOptionalProperty"/>
        <owl:someValuesFrom rdf:resource="https://bamresearch.github.io/bam-masterdata/ControlledName"/>
      </owl:Restriction>
    </rdfs:subClassOf>
    <rdfs:label xml:lang="en">ExampleObjectType</rdfs:label>
    <dc:identifier>EXAMPLE_OBJECT_TYPE</dc:identifier>
    <rdfs:comment xml:lang="en">An example to illustrate how to define an Object Type and its attributes</rdfs:comment>
    <rdfs:comment xml:lang="de">Ein Beispiel zur Veranschaulichung der Definition eines Objekttyps und seiner Attribute</rdfs:comment>
  </owl:Thing>
  <owl:AnnotationProperty rdf:about="http://www.w3.org/2000/01/rdf-schema#comment"/>
  <owl:AnnotationProperty rdf:about="http://purl.org/dc/elements/1.1/identifier"/>
  <owl:Thing rdf:about="https://bamresearch.github.io/bam-masterdata/DatasetType">
    <rdfs:label xml:lang="en">DatasetType</rdfs:label>
  </owl:Thing>
  <owl:AnnotationProperty rdf:about="http://www.w3.org/2000/01/rdf-schema#label"/>
  <owl:ObjectProperty rdf:about="https://bamresearch.github.io/bam-masterdata/hasOptionalProperty">
    <rdfs:range rdf:resource="https://bamresearch.github.io/bam-masterdata/PropertyType"/>
    <rdfs:label xml:lang="en">hasOptionalProperty</rdfs:label>
    <rdfs:comment xml:lang="en">The property is optionally filled when creating the object in openBIS.</rdfs:comment>
  </owl:ObjectProperty>
  <owl:ObjectProperty rdf:about="https://bamresearch.github.io/bam-masterdata/hasMandatoryProperty">
    <rdfs:range rdf:resource="https://bamresearch.github.io/bam-masterdata/PropertyType"/>
    <rdfs:label xml:lang="en">hasMandatoryProperty</rdfs:label>
    <rdfs:comment xml:lang="en">The property must be mandatorily filled when creating the object in openBIS.</rdfs:comment>
  </owl:ObjectProperty>
</rdf:RDF>
